Refine_Imperative_HOL/Lib/Pf_Mono_Prover.thy
@@ -1,7 +1,7 @@
 section {* Interfacing Partial-Function's Monotonicity Prover *}
 theory Pf_Mono_Prover
-imports Separation_Logic_Imperative_HOL.Sep_Main
-begin
+imports Main
+begin                     
   (* TODO: Adjust mono-prover accordingly  *)
   (* Wraps mono-prover of partial-function to erase premises. 
     This is a workaround for mono_tac, which does not accept premises if the case-split rule is applied. *)
